src/invariant/Invariant.v
@@ -21,6 +21,10 @@ Require Import Configuration.
 
 Require Import PromiseConsistent.
 
+Require Import PFStepCommon.
+Require Import PFStep.
+Require Import PFStepCap.
+
 Set Implicit Arguments.
 
 
@@ -181,6 +185,16 @@ Section Invariant.
       + i. esplits; eauto.
   Qed.
 
+  Lemma vals_incl_sem_memory
+        mem1 mem2
+        (VALS: PFStepCommon.vals_incl mem1 mem2)
+        (MEM2: sem_memory mem2):
+    sem_memory mem1.
+  Proof.
+    ii. apply MEM2. ii. specialize (PR loc). des.
+    exploit VALS; eauto.
+  Qed.
+
   Lemma thread_step_sem
         tid lang e
         st1 lc1 sc1 mem1
@@ -194,36 +208,44 @@ Section Invariant.
     <<TH2: S tid lang st2>> /\
     <<MEM2: sem_memory mem2>>.
   Proof.
-    (* inv STEP. *)
-    (* { inv STEP0. symmetry in PF. apply promise_pf_inv in PF. des. subst. *)
-    (*   splits; ss. inv LOCAL. inv PROMISE. *)
-    (*   ii. apply MEM1. ii. specialize (PR loc0). des. *)
-    (*   revert PR. erewrite Memory.lower_o; eauto. condtac; eauto. *)
-    (*   ss. i. des. subst. inv PR. exploit Memory.lower_get0; eauto. i. des. *)
-    (*   inv MSG_LE. eauto. *)
-    (* } *)
-    (* inv STEP0. inv LOCAL. *)
-    (* - esplits; eauto. *)
-    (* - exploit sem_memory_read_step; eauto. i. des. *)
-    (*   exploit READ; eauto. *)
-    (* - exploit WRITE; eauto. i. des. *)
-    (*   esplits; eauto. ii. *)
-    (*   destruct (Const.eq_dec (LocFun.find loc x0) val). *)
-    (*   { subst. hexploit sem_memory_write_step_eq; eauto. i. des. *)
-    (*     rewrite H0. eauto. *)
-    (*   } *)
-    (*   { hexploit sem_memory_write_step_neq; eauto. } *)
-    (* - exploit sem_memory_read_step; eauto. i. des. *)
-    (*   exploit UPDATE; eauto. i. des. *)
-    (*   esplits; eauto. ii. *)
-    (*   destruct (Const.eq_dec (LocFun.find loc x2) valw). *)
-    (*   { subst. hexploit sem_memory_write_step_eq; eauto. i. des. *)
-    (*     rewrite H0. eauto. *)
-    (*   } *)
-    (*   { hexploit sem_memory_write_step_neq; eauto. } *)
-    (* - exploit FENCE; eauto. *)
-    (* - exploit SYSCALL; eauto. *)
-  Admitted.
+    inv STEP.
+    { inv STEP0. inv LOCAL. split; auto.
+      ii. apply MEM1.
+      ii. specialize (PR loc0). des.
+      destruct msg, kind; ss; inv PROMISE.
+      - destruct msg1; ss.
+        revert PR. erewrite Memory.lower_o; eauto. condtac; ss; eauto.
+        des. subst. i. inv PR.
+        exploit Memory.lower_get0; try exact MEM. i. des.
+        inv MSG_LE. eauto.
+      - revert PR. erewrite Memory.add_o; eauto. condtac; ss; eauto.
+      - revert PR. erewrite Memory.split_o; eauto. repeat condtac; ss; eauto.
+        guardH o. des. subst. i. inv PR.
+        exploit Memory.split_get0; eauto. i. des. eauto.
+      - revert PR. erewrite Memory.lower_o; eauto. condtac; ss; eauto.
+    }
+    inv STEP0. inv LOCAL.
+    - esplits; eauto.
+    - exploit sem_memory_read_step; eauto. i. des.
+      exploit READ; eauto.
+    - exploit WRITE; eauto. i. des.
+      esplits; eauto. ii.
+      destruct (Const.eq_dec (LocFun.find loc x0) val).
+      { subst. hexploit sem_memory_write_step_eq; eauto. i. des.
+        rewrite H0. eauto.
+      }
+      { hexploit sem_memory_write_step_neq; eauto. }
+    - exploit sem_memory_read_step; eauto. i. des.
+      exploit UPDATE; eauto. i. des.
+      esplits; eauto. ii.
+      destruct (Const.eq_dec (LocFun.find loc x2) valw).
+      { subst. hexploit sem_memory_write_step_eq; eauto. i. des.
+        rewrite H0. eauto.
+      }
+      { hexploit sem_memory_write_step_neq; eauto. }
+    - exploit FENCE; eauto.
+    - exploit SYSCALL; eauto.
+  Qed.
 
   Lemma rtc_thread_step_sem
         tid lang
@@ -242,6 +264,46 @@ Section Invariant.
     exploit Thread.step_future; eauto. i. des.
     destruct x, y. ss.
     exploit thread_step_sem; eauto. i. des.
+    eapply IHSTEP; eauto.
+  Qed.
+
+  Lemma thread_pf_step_sem
+        tid lang caps
+        st1 lc1 sc1 mem1
+        st2 lc2 sc2 mem2
+        (TH1: S tid lang st1)
+        (MEM1: sem_memory mem1)
+        (WF1: Local.wf lc1 mem1)
+        (SC1: Memory.closed_timemap sc1 mem1)
+        (CLOSED1: Memory.closed mem1)
+        (STEP: PFStepCap.pf_step caps (Thread.mk lang st1 lc1 sc1 mem1) (Thread.mk lang st2 lc2 sc2 mem2)):
+    <<TH2: S tid lang st2>> /\
+    <<MEM2: sem_memory mem2>>.
+  Proof.
+    inv STEP.
+    exploit thread_step_sem; try exact STEP0; eauto. i. des.
+    split; auto.
+    hexploit PFStepCap.lower_cap_vals_incl; eauto. i.
+    eapply vals_incl_sem_memory; eauto.
+  Qed.
+
+  Lemma rtc_thread_pf_step_sem
+        tid lang caps
+        th1 th2
+        (TH1: S tid lang th1.(Thread.state))
+        (MEM1: sem_memory th1.(Thread.memory))
+        (CAPS1: PFStepCap.caps_sound caps th1.(Thread.local).(Local.promises) th1.(Thread.memory))
+        (WF1: Local.wf th1.(Thread.local) th1.(Thread.memory))
+        (SC1: Memory.closed_timemap th1.(Thread.sc) th1.(Thread.memory))
+        (CLOSED1: Memory.closed th1.(Thread.memory))
+        (STEP: rtc (PFStepCap.pf_step caps) th1 th2):
+    <<TH2: S tid lang th2.(Thread.state)>> /\
+    <<MEM2: sem_memory th2.(Thread.memory)>>.
+  Proof.
+    move STEP after TH1. revert_until STEP. induction STEP; ss.
+    i. exploit PFStepCap.pf_step_future; eauto. i. des.
+    destruct x, y. ss.
+    exploit thread_pf_step_sem; eauto. i. des.
     eapply IHSTEP; eauto.
   Qed.
 
@@ -265,92 +327,77 @@ Section Invariant.
         (STEP: Configuration.step e tid c1 c2):
     sem c2.
   Proof.
-    (* inv SEM. econs. *)
-    (* - inv STEP. ss. ii. revert FIND. *)
-    (*   rewrite IdentMap.gsspec. condtac; ss; [|by apply TH]. subst. *)
-    (*   i. inv FIND. apply inj_pair2 in H1. subst. *)
-    (*   eapply rtc_implies in STEPS; [|by apply tau_union]. *)
-    (*   exploit rtc_n1; eauto; i. *)
-    (*   { econs. econs. eauto. } *)
-    (*   exploit Thread.rtc_all_step_future; eauto; ss; try by inv WF. *)
-    (*   { inv WF. eapply WF0. eauto. } *)
-    (*   i. des. *)
-    (*   exploit steps_pf_steps; eauto; ss; try by inv WF. *)
-    (*   { unfold Configuration.consistent in CONSISTENT. ss. *)
-    (*     unfold Threads.consistent in CONSISTENT. *)
-    (*     hexploit CONSISTENT; try eapply IdentMap.gss. i. *)
-    (*     hexploit consistent_promise_consistent; eauto. } *)
-    (*   { inv WF. eapply WF0. eauto. } *)
-    (*   i. des. *)
-    (*   exploit rtc_implies; [|exact STEPS1|i]. *)
-    (*   { apply union_mon. apply Thread.allpf. } *)
-    (*   exploit Thread.rtc_all_step_future; eauto; ss; try by inv WF. *)
-    (*   { inv WF. eapply WF0. eauto. } *)
-    (*   i. des. *)
-    (*   exploit Thread.rtc_step_nonpf_future; eauto. s. i. des. *)
-    (*   subst. eapply rtc_thread_step_sem; try exact STEPS1; eauto; ss; try by inv WF. *)
-    (*   inv WF. eapply WF3. eauto. *)
-    (* - inv STEP. ss. *)
-    (*   assert (WF_LOCAL: Local.wf lc1 (c1.(Configuration.memory))). *)
-    (*   { inv WF. inv WF0. eauto. } *)
-    (*   exploit Thread.rtc_tau_step_future; eauto; try by inv WF. s. i. des. *)
-    (*   exploit Thread.step_future; eauto. s. i. des. *)
-    (*   exploit Memory.no_half_concrete_future_exists; try exact CLOSED0; eauto. *)
-    (*   { apply WF0. } *)
-    (*   i. des. *)
-    (*   unfold Configuration.consistent in CONSISTENT. ss. *)
-    (*   unfold Threads.consistent in CONSISTENT. *)
-    (*   hexploit CONSISTENT; try eapply IdentMap.gss. i. *)
-    (*   exploit H; try exact NOHALF; try refl; eauto; s. *)
-    (*   { inv WF0. econs; eauto. eapply TView.future_closed; eauto. } *)
-    (*   i. des. *)
-    (*   exploit Memory.no_half_concrete_none_future_exists. *)
-    (*   { apply WF_LOCAL. } *)
-    (*   { apply WF. } *)
-    (*   { apply WF. } *)
-    (*   i. des. *)
-    (*   assert (WF_LOCAL': Local.wf lc1 mem0). *)
-    (*   { inv WF_LOCAL. econs; eauto. eapply TView.future_closed; eauto. } *)
-    (*   exploit concrete_none_thread_rtc_tau_step; *)
-    (*     try exact STEPS; try exact CONCRETE0; eauto; try by inv WF. s. i. des. *)
-    (*   exploit concrete_none_thread_step; try exact STEP0; try exact CONCRETE2; eauto. *)
-    (*   { exploit Thread.rtc_tau_step_future; try exact STEPS'; eauto; s. *)
-    (*     { inv WF. eapply Memory.concrete_none_closed_timemap; eauto. } *)
-    (*     i. des. ss. } *)
-    (*   s. i. des. *)
-    (*   exploit Thread.rtc_tau_step_future; try exact STEPS'; eauto; s. *)
-    (*   { inv WF. eapply Memory.future_closed_timemap; eauto. } *)
-    (*   i. des. *)
-    (*   exploit Thread.step_future; try exact STEP'; eauto. s. i. des. *)
-    (*   hexploit Thread.rtc_tau_step_no_half; try exact STEPS'; eauto. s. i. des. *)
-    (*   hexploit Thread.step_no_half; try exact STEP'; eauto. s. i. des. *)
-    (*   exploit LowerMemory.no_half_concrete_none_concrete_lower_memory; *)
-    (*     try exact CONCRETE; try exact CONCRETE1; try exact NOHALF; try apply WF3; eauto. i. *)
-    (*   exploit (@LowerMemory.thread_rtc_tau_step lang (Thread.mk lang st3 lc3 sc3 mem2'0)); *)
-    (*     try exact STEPS0; try refl; eauto; s. *)
-    (*   { inv WF0. econs; eauto. eapply TView.future_closed; eauto. } *)
-    (*   { eapply Memory.future_closed_timemap; try exact SC0; eauto. } *)
-    (*   i. des. *)
-    (*   eapply rtc_implies in STEPS'; [|by apply tau_union]. *)
-    (*   exploit rtc_n1; eauto; i. *)
-    (*   { econs. econs. eauto. } *)
-    (*   eapply rtc_implies in STEPS_SRC; [|by apply tau_union]. *)
-    (*   rewrite STEPS_SRC in x1. *)
-    (*   inv LC2. rewrite PROMISES in PROMISES0. *)
-    (*   exploit steps_pf_steps; try exact x1; eauto; ss; try by inv WF. *)
-    (*   { ii. rewrite PROMISES0, Memory.bot_get in *. congr. } *)
-    (*   { inv WF. eapply Memory.future_closed_timemap; eauto. } *)
-    (*   i. des. *)
-    (*   exploit rtc_union_step_nonpf_bot; eauto. i. subst. *)
-    (*   exploit rtc_thread_step_sem; try exact STEPS1; eauto; ss; try by inv WF. *)
-    (*   { eapply concrete_none_sem_memory; try exact CONCRETE0; eauto. by inv WF. } *)
-    (*   { inv WF. eapply Memory.future_closed_timemap; eauto. } *)
-    (*   i. des. *)
-    (*   exploit Thread.rtc_all_step_future; try exact STEPS0; eauto. s. i. des. *)
-    (*   eapply concrete_sem_memory_inv; try exact CONCRETE2; eauto. *)
-    (*   eapply lower_memory_sem_memory; try exact x0; eauto. *)
-    (*   eapply future_sem_memory; eauto. *)
-  Admitted.
+    inv SEM. econs.
+    - inv STEP. ss. ii. revert FIND.
+      rewrite IdentMap.gsspec. condtac; ss; [|by apply TH]. subst.
+      i. inv FIND. apply inj_pair2 in H1. subst.
+      eapply rtc_implies in STEPS; [|by apply tau_union].
+      exploit rtc_n1; eauto; i.
+      { econs. econs. eauto. }
+      clear STEP0 STEPS COND.
+      inv WF. inv WF0. clear DISJOINT.
+      exploit THREADS; eauto. intro WF. clear THREADS.
+      exploit Thread.rtc_all_step_future; try eapply x0; eauto. s. i. des.
+      exploit (@PFStep.sim_thread_exists
+                 _ (Thread.mk lang0 st1 lc1 c1.(Configuration.sc) c1.(Configuration.memory))); ss.
+      i. des.
+      exploit PFStep.thread_rtc_all_step; try exact SIM; try eapply x0; eauto; ss.
+      { hexploit consistent_promise_consistent; try exact CONSISTENT; ss. }
+      i. des.
+      hexploit PFStep.sim_memory_vals_incl; try eapply SIM; eauto; s; i.
+      { apply WF_SRC. }
+      { apply WF. }
+      hexploit vals_incl_sem_memory; eauto. i.
+      destruct e_src, e2_src. ss. inv SIM. inv SIM2. ss. subst.
+      exploit rtc_thread_step_sem; try exact STEPS_SRC; eauto. i. des. ss.
+    - inv STEP. ss. inv WF. inv WF0. clear DISJOINT.
+      exploit THREADS; eauto. intro WF. clear THREADS.
+      eapply rtc_implies in STEPS; [|by apply tau_union].
+      exploit rtc_n1; eauto.
+      { econs. econs. eauto. }
+      intro STEPS_TGT. clear STEP0 STEPS.
+      exploit Thread.rtc_all_step_future; try exact STEPS_TGT; eauto. s. i. des.
+      exploit Memory.cap_exists; try exact CLOSED2.
+      instantiate (1 := lc3.(Local.promises)). i. des.
+      exploit Memory.cap_closed; eauto. intro CLOSED_CAP.
+      exploit Local.cap_wf; eauto. intro WF_CAP.
+      exploit Memory.max_full_timemap_exists; try eapply CLOSED_CAP. i. des.
+      exploit CONSISTENT; try exact CAP; try exact x0; eauto. s. i. des.
+      exploit (@PFStep.sim_thread_exists
+                 _ (Thread.mk lang st1 lc1 c1.(Configuration.sc) c1.(Configuration.memory))); ss.
+      i. des.
+      exploit PFStep.thread_rtc_all_step; try exact SIM; eauto; ss.
+      { hexploit consistent_promise_consistent; eauto. }
+      i. des.
+      exploit Thread.rtc_all_step_future; try eapply rtc_implies; try exact STEPS_SRC; eauto.
+      { i. inv PR. econs. econs. eauto. }
+      i. des.
+      exploit PFStepCap.sim_thread_exists; try exact SIM2; eauto. s. i. des.
+      exploit PFStepCap.thread_rtc_all_step; try eapply rtc_implies; try exact STEPS; eauto; s.
+      { apply Memory.max_full_timemap_closed; auto. }
+      { i. inv PR. econs. eauto. }
+      { ii. rewrite PROMISES in *. rewrite Memory.bot_get in *. ss. }
+      i. des.
+      exploit Thread.rtc_tau_step_future; try exact STEPS; eauto; s.
+      { eapply Memory.max_full_timemap_closed; eauto. }
+      i. des.
+      hexploit PFStep.sim_memory_vals_incl; try eapply SIM; eauto; s.
+      { apply WF_SRC. }
+      { apply WF. }
+      i. apply vals_incl_sem_memory in H; ss.
+      exploit rtc_thread_step_sem; try exact STEPS_SRC; eauto.
+      { inv SIM. ss. rewrite STATE. eauto. }
+      i. des.
+      hexploit PFStepCap.cap_aux_src_vals_incl; eauto. i.
+      apply vals_incl_sem_memory in H0; ss.
+      exploit rtc_thread_pf_step_sem; try exact STEPS_SRC0; eauto; s.
+      { eapply PFStepCap.sim_memory_caps_sound; eapply SIM0. }
+      i. des.
+      hexploit PFStepCap.sim_memory_bot_vals_incl; try eapply SIM1; eauto. i.
+      apply vals_incl_sem_memory in H1; ss.
+      eapply future_sem_memory; eauto.
+      eapply future_sem_memory; eauto.
+  Qed.
 
   Inductive Configuration_step_evt (c1 c2:Configuration.t): Prop :=
   | Configuration_step_evt_intro
